Removing old implementation

src/CopParser.v
@@ -672,122 +672,20 @@ Example csh_test2 :
 simpl.
 reflexivity. Qed.
 
-Inductive ind_check_sh : (bool * bool) -> Term -> (bool * bool) -> Prop :=
-| csh_asp_sig_t : forall bs bh, (* true case, sign seen previously, no update *)
-                    bs = true -> 
-                    bh = false -> 
-                    ind_check_sh (true, false) (asp SIG) (true, false)
-| csh_asp_sig_f : forall bs bh, (* false case sign not seen previously *)
-                    bs = false ->
-                    ind_check_sh (bs,bh) (asp SIG) (bs,bh)
-| csh_asp_hsh   : forall bh, (* case, sign cannot be seen previously *)
-                    ind_check_sh (false, bh) (asp HSH) (false, bh)
-| csh_asp_other : forall a bs bh, (* other asp's just pass along *)
-                    a <> HSH /\ a <> SIG -> 
-                    (* TODO: Technically think we allow (true,true) now, but not reachable? *)
-                    ind_check_sh (bs,bh) (asp a) (bs,bh)
-| 
-
-Example ind_check_sh1 : ind_check_sh (true, false) (asp SIG) (true, false).
-apply (csh_asp_sig_t true false); reflexivity. Qed.
-
-Example ind_check_sh2 : ~ (ind_check_sh (true, false) (asp HSH) (true, true)).
-(* we cannot generate a failing program *)
-unfold not. intros.
-qinv H. Qed.
-
-Example ind_check_sh3 : forall b1 b2, (ind_check_sh (b1, b2) (asp CPY) (b1,b2)).
-constructor.
-split; intros H; discriminate.
-Qed.
-
-    match t with
-    | (asp a) =>
-        match a with
-        | SIG => let (s', h') := bb in if s' then (s', h') else (true, false)
-        | HSH => let (s', _) := bb in (s', true)
-        | _ => (false, false)
-        end
-    | (att plc t)            => checkSign_Hash bb t
-    | (lseq f sec)            => match (checkSign_Hash bb f) with
-                                | (sf,hf) => if sf
-                                                then (if hf 
-                                                    then (true,true)
-                                                    else (checkSign_Hash (sf,hf) sec))
-                                                else (checkSign_Hash (sf,hf) sec)
-                                end
-    | (bseq (sp1,sp2) f sec) => match sp1 with
-                                | ALL => match sp2 with
-                                        | ALL => (* Check both*)
-                                            match (checkSign_Hash bb f) with
-                                            | (true, true)  => (true,true)
-                                            | (sf,hf)       => (checkSign_Hash (sf,hf) sec)
-                                            end
-                                        | NONE => (* Check only sp1 with above, reset below*)
-                                            match (checkSign_Hash bb f) with
-                                            | (true, true)  => (true,true)
-                                            | (sf,hf)    => (checkSign_Hash (false,false) sec)
-                                            end
-                                        end
-                                | NONE => match sp2 with
-                                        | ALL => (* Check only sp2 with above, reset below*)
-                                            match (checkSign_Hash (false,false) f) with
-                                            | (true, true)  => (true,true)
-                                            | (sf,hf)       => (checkSign_Hash bb sec)
-                                            end
-                                        | NONE => (* reset for both*)
-                                            match (checkSign_Hash (false,false) f) with
-                                            | (true, true)  => (true,true)
-                                            | (sf,hf)       => (checkSign_Hash (false,false) sec)
-                                            end
-                                        end
-                                end
-    | (bpar (sp1,sp2) f sec) => match sp1 with
-                                | ALL => match sp2 with
-                                        | ALL => (* Check both*)
-                                            match (checkSign_Hash bb f) with
-                                            | (true, true)  => (true,true)
-                                            | (sf,hf)       => (checkSign_Hash (sf,hf) sec)
-                                            end
-                                        | NONE => (* Check only sp1 with above, reset below*)
-                                            match (checkSign_Hash bb f) with
-                                            | (true, true)  => (true,true)
-                                            | (sf,hf)       => (checkSign_Hash (false,false) sec)
-                                            end
-                                        end
-                                | NONE => match sp2 with
-                                        | ALL => (* Check only sp2 with above, reset below*)
-                                            match (checkSign_Hash (false,false) f) with
-                                            | (true, true)  => (true,true)
-                                            | (sf,hf)       => (checkSign_Hash bb sec)
-                                            end
-                                        | NONE => (* reset for both*)
-                                            match (checkSign_Hash (false,false) f) with
-                                            | (true, true)  => (true,true)
-                                            | (sf,hf)       => (checkSign_Hash (false,false) sec)
-                                            end
-                                        end
-                                end 
-    end.
-
-Inductive Option {X : Type} : Type :=
-| Some {X} (n : X)
-| None.
-
-Definition sign_hash_TypeCheck (t : Term) : @Option Term :=
+Definition sign_hash_TypeCheck (t : Term) : @optionE Term :=
     match (checkSign_Hash (false,false) t) with
-    | (true, true)  => None
-    | (_,_)         => Some t
+    | (true, true)  => NoneE "Failed typecheck"
+    | (_,_)         => SomeE t
     end.
 
-Example shTC1 : sign_hash_TypeCheck (lseq (asp SIG) (asp HSH)) = None.
+Example shTC1 : sign_hash_TypeCheck (lseq (asp SIG) (asp HSH)) = NoneE "Failed typecheck".
 Proof. reflexivity. Qed.
 
-Example shTC2 : sign_hash_TypeCheck (lseq (asp HSH) (asp SIG)) = Some (lseq (asp HSH) (asp SIG)).
+Example shTC2 : sign_hash_TypeCheck (lseq (asp HSH) (asp SIG)) = SomeE (lseq (asp HSH) (asp SIG)).
 reflexivity. Qed.
 
 Lemma none_not_some : forall (t : Term),
-    @None Term = Some t -> False.
+    @NoneE Term "" = SomeE t -> False.
 Proof.
     intros. discriminate.
 Qed.
@@ -814,8 +712,8 @@ Proof.
 Qed.
 
 Lemma att_injective_SH : forall p t,
-    sign_hash_TypeCheck (att p t) = Some (att p t) ->
-    sign_hash_TypeCheck t = Some t.
+    sign_hash_TypeCheck (att p t) = SomeE (att p t) ->
+    sign_hash_TypeCheck t = SomeE t.
 Proof.
     unfold sign_hash_TypeCheck.
     intros.
@@ -936,143 +834,5 @@ Proof.
         * qinv H0. apply H3.
         * qinv H0. apply H3.
 Qed.
-
-Theorem checkSH_impl_not_hash_sig_term : forall (t : Term),
-    sign_hash_TypeCheck t = Some t ->
-    not_hash_sig_term t.
-Proof.
-    intros t H.
-    unfold sign_hash_TypeCheck in H. 
-    unfold not_hash_sig_term.
-    induction t; simpl in *; unfold not in *.
-    - admit.
-    - intros t' Ht' Htsub. 
-      destruct (checkSign_Hash (false,false) t) eqn:E.
-      destruct b,b0; simpl in *; try discriminate.
-      * assert (Htemp : @Some Term Term t = Some t). {
-          reflexivity.
-      } apply (IHt Htemp (att p t)). 
-        qinv Htsub.
-        ** assumption.
-    Restart.
-    intros t H.
-    induction t; unfold not_hash_sig_term in *; unfold not in *; simpl in *; intros.
-    - qinv H1. qinv H0. destruct H1 as [e [H1 [H2 H3]]].
-        qinv H1.
-    - pose proof (att_injective_SH p t). apply H2 in H. 
-        apply (IHt H t').
-        * apply H0.
-        * pose proof (att_term_sub_bijection t t' p).
-            apply H3.
-            ** unfold not. intros. (* possible they equal, but violate hash_sig *)
-                subst. qinv H0.
-                destruct H4 as [e [He1 [He2 He3]]].
-                discriminate.
-            ** apply H1.
-    - 
-
-Theorem not_hash_sig_term_impl_typeCheckPass: 
-    forall (t : Term),
-        not_hash_sig_term t -> sign_hash_TypeCheck t = Some t.
-Proof.
-    intros t H.
-    unfold not_hash_sig_term in H.
-    induction t.
-    - (* basic asp *)
-        induction a; reflexivity.
-    - (* basic att *)
-        unfold sign_hash_TypeCheck in *.
-        pose proof (none_not_some t) as NTF.
-        destruct (checkSign_Hash (false,false) (att p t)) eqn:E;
-        destruct (checkSign_Hash (false,false) t) eqn:E'.
-        destruct b,b0; try reflexivity.
-        destruct b1,b2; simpl in *.
-        * exfalso. apply NTF.
-            apply IHt.
-            intros.
-            specialize H with t'.
-            unfold not. intros. 
-            apply H. apply H0.
-            apply aatt_sub_annt. apply H1.
-        * rewrite E in E'. discriminate.
-        * rewrite E in E'. discriminate.
-        * rewrite E in E'. discriminate.
-    - (* lseq t1 t2*)
-        unfold sign_hash_TypeCheck in *.
-        destruct (checkSign_Hash (false,false) t1) eqn:Et1.
-        destruct (checkSign_Hash (false,false) t2) eqn:Et2.
-        (* We should be able to construct Lt1t2 from previous *)
-        (* destruct (checkSign_Hash (false,false) (lseq t1 t2)) eqn:Lt1t2. *)
-        (* destruct b3,b4; try reflexivity. *)
-        destruct b,b0; destruct b1,b2; try (
-            (* kill t1 cases *)
-            exfalso;
-            apply (none_not_some (t1));
-            apply IHt1; intros;
-            specialize H with t';
-            unfold not; intros;
-            apply H; [apply H0 | apply alseq_subl_annt; apply H1]
-        ); try (
-            (* kill t2 cases *)
-            exfalso;
-            apply (none_not_some (t2));
-            apply IHt2; intros;
-            specialize H with t';
-            unfold not; intros;
-            apply H; [apply H0 | apply alseq_subr_annt; apply H1]
-        ).
-        * pose proof (checkSH_lseq t2 t1 true false) as Hsh.
-            destruct Hsh as [_ Hsh].
-            apply Hsh in Et2.
-            ** 
-            ** 
-        * qinv Lt1t2. rewrite Et1 in H1.
-            (* even if we start in true we never see HSH to double true *)
-            admit.
-        * qinv Lt1t2. rewrite Et1 in H1.
-            (* this is very tricky, seems like it should truly be false *)
-            admit.
-        * qinv Lt1t2. rewrite Et1 in H1.
-            (* never see HSH *)
-            admit.
-        * qinv Lt1t2. rewrite Et1 in H1.
-            (* tricky case, seems like should fail *)
-            admit.
-        * rewrite <- Et1 in Et2. qinv Lt1t2.
-            rewrite Et1 in H1.
-            admit.
-
-
-        (* either works *)
-        * exfalso. 
-            apply (none_not_some (t2)).
-            apply IHt2. unfold not. intros.
-            specialize H with t'.
-            apply H.
-            ** apply H0.
-            ** apply alseq_subr_annt. apply H1.
-        (* only t1 works *)
-        * exfalso. 
-            apply (none_not_some (t1)).
-            apply IHt1. intros.
-            specialize H with t'.
-            unfold not. intros.
-            apply H.
-            ** apply H0.
-            ** apply alseq_subl_annt. apply H1.
-        (* only t1 works *)
-        * exfalso. 
-            apply (none_not_some (t1)).
-            apply IHt1. intros.
-            specialize H with t'.
-            unfold not. intros.
-            apply H.
-            ** apply H0.
-            ** apply alseq_subl_annt. apply H1.
-        * 
-
-    
-Qed.
-
 
 End CopParser.
